\appendix
\chapter{Pagalbinės formulės uždaviniams spręsti}

\section{Ribų skaičiavimo formulės}

\begin{align} 
%
  &\lim_{x \to 0} \frac{\sin x}{x} = 1
  \label{f_lim_sin} \\
%
  &\lim_{x \to 0} \left( 1 + x \alpha \right)^{\frac{1}{x}} = e^{\alpha}
  \label{f_lim_exp} \\
%
  &\lim_{x \to 0} \frac{a^x - 1}{x} = \ln a, 
  & \text{ kur } a > 0, a \neq 1
  \label{f_lim_ep} \\
% 
  &\lim_{x \to 0} \frac{(1 + x)^r -1}{x} = r, & \text{ kur } r \in \RSET
  \label{f_lim_lp} \\
%
  &\lim_{x \to 0} \frac{\log _{a} (1 + x)}{x} = \log _{a} e, 
  & \text{ kur } a > 0, a \neq 1
  \label{f_lim_log} \\
%
  &\lim_{x \to +\infty} \frac{a^x}{x^r} = +\infty, 
  & \text{ kur } a > 1, r \in \RSET
  \label{f_lim_rl} \\
% 
  &\lim_{x \to +\infty} \frac{\log _{a} x}{x^r} = 0,
  & \text{ kur } a > 1, r > 0
  \label{f_lim_llb} \\
%
  &\lim_{x \to 0} x^p \log _{a} x = 0, & \text{ kur } a > 1, p > 0
  \label{f_lim_lln}
%
\end{align}

\section{Trigonometrinės tapatybės}

\begin{align}
%
  & \sin ^{2} \alpha + \cos ^{2} \alpha = 1
  \label{f_tri_kvsum} \\
%
  & \sin \alpha - \sin \beta = 2 
    \sin \left( \frac{\alpha - \beta}{2} \right)
    \cos \left( \frac{\alpha + \beta}{2} \right)
  \label{f_tri_sinsk} \\
%
  & \cos 2 \alpha = \cos ^{2} \alpha - \sin ^{2} \alpha
  \label{f_tri_dkcos} \\
%
  & \sin (\alpha + \beta) = 
  \sin (\alpha) \cos (\beta) + \cos(\alpha) \sin(\beta) 
  \label{f_tri_sin} \\
  & \sin 2 \alpha = 2 \sin \alpha \cos \alpha
  \label{f_tri_dksin} 
%
\end{align}

\section{Elementarių funkcijų išvestinės}

\label{dx_formulynas}

\begin{align}
%
  (x^{\alpha})' &= \alpha x^{\alpha - 1}
  \label{dx_laipsnine} \\
%
  (\sin x)' &= \cos x
  \label{dx_sin} \\
%
  (\cos x)' &= - \sin x
  \label{dx_cos} \\
%
  (\tg x)' &= \frac{1}{\cos^{2} x}
  \label{dx_tg} \\
%
  (\ctg x)' &= \frac{1}{\sin^{2} x}
  \label{dx_ctg} \\
%
  (\arcsin x)' &= \frac{1}{\sqrt{1 - x^{2}}}
  \label{dx_arcsin} \\
%
  (\arccos x)' &= - \frac{1}{\sqrt{1 - x^{2}}}
  \label{dx_arccos} \\
%
  (\arctg x)' &= \frac{1}{1 + x^{2}}
  \label{dx_arctg} \\
%
  (\arcctg x)' &= - \frac{1}{1 + x^{2}}
  \label{dx_arcctg} \\
%
  (a^{x})' &= a^{x} \cdot \ln a
  \label{dx_expo} \\
%
  (\log _{a} x)' &= \frac{1}{x \cdot \ln a}
  \label{dx_log} \\
%
  (\sinh x)' &= \cosh x
  \label{dx_sh} \\
%
  (\cosh x)' &= \sinh x
  \label{dx_ch} \\
% 
  (\tanh x)' &= \frac{1}{\cosh^{2} x}
  \label{dx_th} \\
%
  (\coth x)' &= \frac{1}{\sinh^{2} x}
  \label{dx_cth}
\end{align}

\begin{note}
  \begin{align*}
    \sinh x &:= \frac{e^{x} - e^{-x}}{2} \\
    \cosh x &:= \frac{e^{x} + e^{-x}}{2} \\
    \tanh x &:= \frac{\sinh x}{\cosh x} \\
    \coth x &:= \frac{\cosh x}{\sinh x}
  \end{align*}
\end{note}
